Made put__inner mostly; need to give a persistent has_gokv_encoding fact
in the postcondition, so we can know that the logical state of the aof
matches the current volatile state of the server.

also fixed missing code that updates the reply table before responding.

external/Goose/github_com/mit_pdos/gokv/goosekv.v
@@ -41,7 +41,10 @@ Definition GoKVServer__put_inner: val :=
   rec: "GoKVServer__put_inner" "s" "args" "reply" :=
     (if: lockservice.CheckReplyTable (struct.loadF GoKVServer.S "lastSeq" "s") (struct.loadF GoKVServer.S "lastReply" "s") (struct.loadF lockservice.RPCRequest.S "CID" "args") (struct.loadF lockservice.RPCRequest.S "Seq" "args") "reply"
     then #()
-    else MapInsert (struct.loadF GoKVServer.S "kvs" "s") (struct.get lockservice.RPCVals.S "U64_1" (struct.loadF lockservice.RPCRequest.S "Args" "args")) (struct.get lockservice.RPCVals.S "U64_2" (struct.loadF lockservice.RPCRequest.S "Args" "args"))).
+    else
+      MapInsert (struct.loadF GoKVServer.S "kvs" "s") (struct.get lockservice.RPCVals.S "U64_1" (struct.loadF lockservice.RPCRequest.S "Args" "args")) (struct.get lockservice.RPCVals.S "U64_2" (struct.loadF lockservice.RPCRequest.S "Args" "args"));;
+      struct.storeF lockservice.RPCReply.S "Ret" "reply" #0;;
+      MapInsert (struct.loadF GoKVServer.S "lastReply" "s") (struct.loadF lockservice.RPCRequest.S "CID" "args") #0).
 
 Definition GoKVServer__Put: val :=
   rec: "GoKVServer__Put" "s" "args" "reply" :=
