src/program_proof/lockservice/gokv_proof.v
@@ -101,7 +101,8 @@ Definition gokv_inv s γ : iProp Σ :=
 Definition is_gokvserver s γ : iProp Σ :=
   ∃ mu,
   "#Hmu" ∷ readonly (s ↦[GoKVServer.S :: "mu"] mu) ∗
-  "#Hmu_inv" ∷ is_lock goKVN mu (gokv_inv s γ)
+  "#Hmu_inv" ∷ is_lock goKVN mu (gokv_inv s γ) ∗
+  "#His_rpc" ∷ is_RPCServer γ.(rpc_gn)
 .
 
 Definition reply_res γrpc req (reply:@RPCReply u64) : iProp Σ :=
@@ -150,8 +151,11 @@ Lemma wp_encodeReq_put req_ptr rid args :
 Proof.
 Admitted.
 
-Lemma wp_GoKVServer__put_inner s req_ptr reply_ptr rid args gkv reply :
-  ∃ gkv',
+Lemma wp_GoKVServer__put_inner γ s req_ptr reply_ptr rid args gkv reply γreq:
+∃ gkv',
+is_RPCServer γ.(rpc_gn) -∗
+is_RPCRequest γ.(rpc_gn) γreq (∃ oldv, args.(U64_1) [[γ.(kvs_gn)]]↦ oldv)
+      (λ v : u64, args.(U64_1) [[γ.(kvs_gn)]]↦ args.(U64_2)) rid -∗
   {{{
        read_request req_ptr rid args ∗
        own_reply reply_ptr reply ∗
@@ -160,7 +164,7 @@ Lemma wp_GoKVServer__put_inner s req_ptr reply_ptr rid args gkv reply :
     GoKVServer__put_inner #s #req_ptr #reply_ptr
   {{{
        reply', RET #(); gokv_core s gkv' ∗
-            (∀ data req_data γ, has_gokv_encoding data gkv →
+            (∀ data req_data, has_gokv_encoding data gkv →
                               ⌜has_req_encoding_put req_data rid args⌝ →
                               gokv_aof_ctx γ.(rpc_gn) γ.(kvs_gn) (data) ={⊤}=∗
                               gokv_aof_ctx γ.(rpc_gn) γ.(kvs_gn) (data ++ req_data) ∗ reply_res γ.(rpc_gn) rid reply' (* this should be resources for the reply' *)
@@ -171,8 +175,9 @@ Lemma wp_GoKVServer__put_inner s req_ptr reply_ptr rid args gkv reply :
 Proof.
   destruct (wp_CheckReplyTable gkv.(lastSeqM) gkv.(lastReplyM) rid) as [b H].
   eexists (if b then _ else _).
+  iIntros "#His_rpc #HreqInv".
   iLöb as "IH" forall (s req_ptr reply_ptr reply).
-  iIntros (Φ) "Hpre HΦ".
+  iIntros (Φ) "!# Hpre HΦ".
   wp_lam.
   wp_pures.
   iDestruct "Hpre" as "(#Hargs & Hreply & Hcore)".
@@ -199,7 +204,7 @@ Proof.
       iExists _, _, _, _. iFrame "#∗".
     }
     {
-      iFrame. iIntros (???) "#Henc1". iIntros (?) "Hctx".
+      iFrame. iIntros (??) "#Henc1". iIntros (?) "Hctx".
       iNamed "Hctx".
       iDestruct (has_gokv_encoding_injective with "Henc1 Henc") as %<-.
       iDestruct ("Hwand" with "Hsrpc") as "#Hres".
@@ -235,9 +240,18 @@ Proof.
   wp_apply (wp_MapInsert with "HkvsMap").
   { done. }
   iIntros "HkvsMap".
+  wp_pures.
+  iDestruct "Hreply" as "(H1 & H2)".
+  iNamed "H1". iNamed "H2".
+  wp_storeField.
+  wp_loadField.
+  wp_loadField.
+  wp_apply (wp_MapInsert with "HlastReply").
+  { done. }
+  iIntros "HlastReplyMap".
 
   iApply "HΦ".
-  iSplitR "Hreply".
+  iSplitR "HReplyOwnRet HReplyOwnStale".
   {
     instantiate (1:= mkGoKVServerC _ _ _).
     iExists _, _, _, _.
@@ -246,7 +260,8 @@ Proof.
     iFrame "HlastSeqOwn HlastReplyOwn HkvsOwn ∗".
   }
   {
-    iFrame. iIntros (???) "#Henc1". iIntros (?) "Hctx".
+    instantiate (1:=Build_RPCReply _ (U64 0)). iFrame.
+    iIntros (??) "#Henc1". iIntros (?) "Hctx".
     iNamed "Hctx".
     iDestruct (has_gokv_encoding_injective with "Henc1 Henc") as %<-.
     rewrite sep_exist_r.
@@ -268,18 +283,39 @@ Proof.
     }
     iSimpl.
     (* TODO: want rpc request invariant here*)
-    admit.
-  }
-Admitted.
+    iMod (server_takes_request with "HreqInv Hsrpc") as "(Hγpre & HcorePre & Hprocessing)".
+    { done. }
+    { lia. }
+    iMod "HcorePre".
+    iNamed "HcorePre".
+    iMod (map_update with "Hghost HcorePre") as "[Hghost Hptsto]".
+    Transparent typed_map.map_insert.
+    iFrame "Hghost".
+    iMod (server_completes_request with "His_rpc HreqInv Hγpre Hptsto Hprocessing") as "[#Hreceipt Hsrpc] /=".
+    { done. }
+    { done. }
+    { apply Z.gt_lt. unfold u64. done. }
 
-Lemma wp_GoKVServer__Put (s:loc) va γ :
+    replace ((let (_, lastReplyM0, _) := gkv in lastReplyM0)) with (gkv.(lastReplyM)) by done.
+    iSimpl.
+    iFrame "Hsrpc".
+    iRight.
+    iFrame "Hreceipt".
+    by iModIntro.
+  }
+  Unshelve.
+  { done. }
+  { done. }
+Qed.
+
+Lemma wp_GoKVServer__Put (s:loc) γ :
 is_gokvserver s γ -∗
   {{{
        True
   }}}
     GoKVServer__Put #s
   {{{ (f:goose_lang.val), RET f;
-        ∀ args req, is_rpcHandler f γ.(rpc_gn) args req (args.(U64_1) [[γ.(kvs_gn)]]↦ va) (λ v, ⌜v = va⌝ ∗ args.(U64_1) [[γ.(kvs_gn)]]↦ v)
+        ∀ args req, is_rpcHandler f γ.(rpc_gn) args req (∃ oldv, args.(U64_1) [[γ.(kvs_gn)]]↦ oldv) (λ _, args.(U64_1) [[γ.(kvs_gn)]]↦ args.(U64_2))
   }}}.
 Proof.
   iIntros "#Hls".
@@ -300,18 +336,19 @@ Proof.
 
   wp_pures.
 
-  wp_apply (wp_GoKVServer__put_inner with "[$Hargs $Hreply $Hcore]").
-  iIntros (gkv' reply') "(Hcore & HcommitFupd & Hreply)".
+  edestruct (wp_GoKVServer__put_inner) as [gkv' H].
+  wp_apply (H with "His_rpc HargsInv [$Hargs $Hreply $Hcore]").
+  iIntros (reply') "(Hcore & HcommitFupd & Hreply)".
   wp_pures.
 
   wp_apply (wp_encodeReq_put with "[$Hargs]").
   iIntros (req_sl req_data) "[Hreq_sl %Hreq_enc]".
   wp_loadField.
-  iDestruct "Haof_log" as (?) "[Haof_log %]".
+  iDestruct "Haof_log" as (?) "[Haof_log #Henc]".
   wp_apply (wp_AppendOnlyFile__Append with "His_aof [$Hreq_sl $Haof_log HcommitFupd]").
   {
     iIntros "Hctx".
-    iMod ("HcommitFupd" $! data req_data γ with "[] [] Hctx") as "Hfupd".
+    iMod ("HcommitFupd" $! data req_data with "[] [] Hctx") as "Hfupd".
     { done. }
     { done. }
     iFrame.
@@ -339,3 +376,5 @@ Proof.
   iApply "HΦ".
   iExists _; iFrame "∗#".
 Admitted.
+
+End gokv_proof.
